Finish refactoring substitution

IMLTT/Substitution.lean
@@ -1,67 +1,175 @@
-import IMLTT.AbstractSyntax 
+import IMLTT.AbstractSyntax
 
--- FIXME: subsitute, lift in type annotations? e.g. in j
+-- ASTs
 
-/- # Lifting -/
--- needed to preserver `original depth` of variables
--- -> free variables need to refer to same context entry or constant
--- currently according to Abel and colleagues (2007)
-def lift (l j : Nat) : Tm -> Tm
+-- TODO: is it possibe to readd comp?
+inductive Weak where
+  | id : Weak
+  | shift : Weak → Weak
+  | lift : Weak → Weak
+
+inductive Subst where
+  | weak : Weak → Subst
+  | shift : Subst → Subst
+  | lift : Subst → Subst
+  | extend : Subst → Tm → Subst
+
+-- AST → AST
+
+def comp_weaken (ρ ρ' : Weak) : Weak :=
+  match ρ with
+  | .id => ρ'
+  | .shift γ => .shift (comp_weaken γ ρ')
+  | .lift γ  =>
+    match ρ' with
+    | .id => .lift γ
+    | .shift γ' => .shift (comp_weaken γ γ')
+    | .lift γ' => .lift (comp_weaken γ γ')
+
+def subst_from_list (ts : List Tm) : Subst :=
+  match ts with
+  | [] => .weak .id
+  | t :: ts' => .extend (subst_from_list ts') t
+
+-- weakening: Nat → Nat
+
+def id_weak : Nat → Nat :=
+  id
+
+def shift_weak (ρ : Nat → Nat) : Nat → Nat :=
+  fun i ↦ ρ i + 1
+
+def lift_weak (ρ : Nat → Nat) : Nat → Nat :=
+  fun i ↦
+    match i with 
+    | 0 => 0
+    | i' + 1 => (ρ i') + 1
+
+def parse_weak (ρ : Weak) : Nat → Nat :=
+  match ρ with
+  | .id => id_weak
+  | .shift ρ => shift_weak (parse_weak ρ)
+  | .lift ρ => lift_weak (parse_weak ρ)
+
+def lift_weak_n (j : Nat) (ρ : Nat → Nat) : Nat → Nat
+  | i =>
+    match j with
+    | 0 => ρ i
+    | j' + 1 => (lift_weak_n j' ρ) i
+
+def weak (t : Tm) (ρ : Nat → Nat) : Tm :=
+  match t with
   | .unit => .unit
   | .empty => .empty
-  | .pi A B  => .pi (lift l j A) (lift (l + 1) j B)
-  | .sigma A B => .sigma (lift l j A) (lift (l + 1) j B)
-  | .iden A s t => .iden (lift l j A) (lift l j s) (lift l j t)
+  | .pi A B => .pi (weak A ρ) (weak B (lift_weak_n 1 ρ))
+  | .sigma A B => .sigma (weak A ρ) (weak B (lift_weak_n 1 ρ))
+  | .iden A a a' => .iden (weak A ρ) (weak a ρ) (weak a' ρ)
   | .univ => .univ
-  | .var i =>
-      if i < l
-        then .var i
-        else .var (i + j)
+  | .var i => ρ i
   | .tt => .tt
-  | .indUnit A s t => .indUnit (lift l j A) (lift l j s) (lift l j t)
-  | .indEmpty A s => .indEmpty (lift l j A) (lift l j s)
-  | .lam s t => .lam (lift l j s) (lift (l + 1) j t)
-  | .app s t => .app (lift l j s) (lift l j t)
-  | .pairSigma s t => .pairSigma (lift l j s) (lift (l + 1) j t)
-  | .indSigma A B C s t => .indSigma (lift l j A) (lift l j B) (lift l j C) 
-                            (lift l j s) (lift l j t)
-  | .refl A t => .refl (lift l j A) (lift l j t)
-  | .j A B t a b p => .j (lift l j A) (lift l j B) (lift l j t) (lift l j a) (lift l j b) (lift l j p)
+  | .indUnit A b a => .indUnit (weak A (lift_weak_n 1 ρ)) (weak b ρ) (weak a ρ)
+  | .indEmpty A b => .indEmpty (weak A (lift_weak_n 1 ρ)) (weak b ρ)
+  | .lam A b => .lam (weak A ρ) (weak b (lift_weak_n 1 ρ))
+  | .app f a => .app (weak f ρ) (weak a ρ)
+  | .pairSigma a b => .pairSigma (weak a ρ) (weak b (lift_weak_n 1 ρ))
+  | .indSigma A B C c p => .indSigma (weak A ρ) (weak B (lift_weak_n 1 ρ)) (weak C (lift_weak_n 1 ρ))
+                            (weak c (lift_weak_n 2 ρ)) (weak p ρ)
+  | .refl A a => .refl (weak A ρ) (weak a ρ)
+  | .j A B b a a' p => .j (weak A ρ) (weak B (lift_weak_n 3 ρ)) (weak b (lift_weak_n 1 ρ))
+                        (weak a ρ) (weak a' ρ) (weak p ρ)
 
--- TODO: use more efficient lifting
--- - on λ-calculus (ex3) lecture only apply lifting when really substituted
+def weaken (t : Tm) (ρ : Weak) : Tm :=
+  weak t (parse_weak ρ)
 
-/- # Substitution -/
--- lifting used
--- decrease var that references binder outside the length of the substitution
-def substitute (s : Tm) (t : Tm) (j : Nat) : Tm :=
-  match s with
-  | .unit => .unit
-  | .empty => .empty
-  | .pi A B  => .pi (substitute A t j) (substitute B (lift 0 1 t) (j + 1))
-  | .sigma A B => .sigma (substitute A t j) (substitute B (lift 0 1 t) (j + 1))
-  | .iden A m n => .iden A (substitute m t j) (substitute n t j)
-  | .univ => .univ
-  | .var i =>
-      if i < j
-        then .var i
-        else if i = j
-          then t
-          else .var (i - 1)
-  | .tt => .tt
-  | .indUnit A m n => .indUnit (substitute A t j) (substitute m t j) (substitute n t j)
-  | .indEmpty A m => .indEmpty (substitute A t j) (substitute m t j)
-  | .lam m n => .lam (substitute m t j) (substitute n (lift 0 1 t) (j + 1))
-  | .app m n => .app (substitute m t j) (substitute n t j)
-  | .pairSigma m n => .pairSigma (substitute m t j) (substitute n (lift 0 1 t) (j + 1))
-  | .indSigma A B C m n => .indSigma (substitute A t j) (substitute B t j) (substitute C t j) 
-                            (substitute m t j) (substitute n t j)
-  | .refl A m => .refl (substitute A t j) (substitute m t j)
-  | .j A B u a b p => .j (substitute A t j) (substitute B t j) (substitute u t j) (substitute a t j) 
-                      (substitute b t j) (substitute p t j)
+def comp_weak (ρ ρ' : Nat → Nat) : Nat → Nat
+  | i => ρ (ρ' i)
 
-notation A "[" t  "/" j"]" => substitute A t j
+-- helpers
 
-def lift_ctx (l j : Nat) : Ctx -> Ctx
-  | .empty => .empty
-  | .extend Γ A => .extend (lift_ctx l j Γ) (lift l j A)
+def weak_var (i : Nat) (ρ : Weak) : Nat :=
+  (parse_weak ρ) i
+
+def shift_tm : Tm → Tm
+  | t => weaken t (.shift .id)
+
+def parse_weak_to_sub (ρ : Nat → Nat) : Nat → Tm
+  | i => .var (ρ i)
+
+def id_subst : Nat → Tm :=
+  .var
+
+-- substitution: Nat → Tm
+
+def shift_tm_f : Tm → Tm
+  | t => weak t (parse_weak (.shift .id))
+
+def shift_subst (σ : Nat → Tm) : Nat → Tm
+  | i => shift_tm_f (σ i)
+
+def lift_subst (σ : Nat → Tm) : Nat → Tm
+  | 0 => 0
+  | i + 1 => shift_subst σ i
+
+def extend_subst (σ : Nat → Tm) (t : Tm) : Nat → Tm
+  | 0 => t
+  | (i + 1) => σ i
+
+mutual
+  def comp_subst (σ σ' : Nat → Tm) : Nat → Tm
+    | i => sub (σ' i) σ
+
+  def parse_subst (σ : Subst) : Nat → Tm :=
+    match σ with
+    | .weak ρ => parse_weak_to_sub (parse_weak ρ)
+    | .shift σ => shift_subst (parse_subst σ)
+    | .lift σ => lift_subst (parse_subst σ)
+    | .extend σ t => extend_subst (parse_subst σ) t
+
+  def sub (t : Tm) (σ : Nat → Tm) : Tm :=
+    match t with
+    | .unit => .unit
+    | .empty => .empty
+    | .pi A B => .pi (sub A σ) (sub B (lift_subst σ))
+    | .sigma A B => .sigma (sub A σ) (sub B (lift_subst σ))
+    | .iden A a a' => .iden (sub A σ) (sub a σ) (sub a' σ)
+    | .univ => .univ
+    | .var i => σ i
+    | .tt => .tt
+    | .indUnit A b a => .indUnit (sub A (lift_subst σ)) (sub b σ) (sub a σ)
+    | .indEmpty A b => .indEmpty (sub A (lift_subst σ)) (sub b σ)
+    | .lam A b => .lam (sub A σ) (sub b (lift_subst σ))
+    | .app f a => .app (sub f σ) (sub a σ)
+    | .pairSigma a b => .pairSigma (sub a σ) (sub b (lift_subst σ))
+    | .indSigma A B C c p => .indSigma (sub A σ) (sub B (lift_subst σ)) 
+                              (sub C (lift_subst σ)) (sub c (lift_subst (lift_subst σ)))
+                              (sub p σ) -- FIXME: Σ-comp is wrong - last assumption
+    | .refl A a => .refl (sub A σ) (sub a σ)
+    | .j A B b a a' p => .j (sub A σ) (sub B (lift_subst (lift_subst (lift_subst σ))))
+                          (sub b (lift_subst σ)) (sub a σ) (sub a' σ)
+                          (sub p σ) -- FIXME: j-rule is wrong
+end
+
+def substitute (t : Tm) (σ : Subst) : Tm :=
+  sub t (parse_subst σ)
+
+def parse_weak_comp (ρ : Weak) (σ : Subst) : Nat → Tm
+  | i => weaken ((parse_subst σ) i) ρ
+
+def subst_weak_comp (σ : Subst) (ρ : Weak) : Nat → Tm
+  | i => (parse_subst σ) (weak_var i ρ)
+
+-- helpers:
+def substitute_zero (t : Tm) (a : Tm) : Tm :=
+  substitute t (.extend (.weak .id) a)
+
+notation "id" => Weak.id
+notation "↑" => Weak.shift
+notation "⇑" => Weak.lift
+notation "⇑_" i => lift_weak_n i
+notation ρ "∘" ρ' => comp_weaken ρ ρ'
+notation A "[" ρ "]" => weaken A ρ
+
+notation "↑" => Subst.shift
+notation "⇑" => Subst.lift
+notation σ "∘" σ' => Subst.comp σ σ'
+notation A "[" σ "]" => substitute A σ
